working on proving execute stage of pipelined vs multicycle

example/out/ProcMemSpec.v
@@ -16,11 +16,13 @@ Definition AddrSz := 32.
 
 Definition InstrSz := 32.
 
-Notation NumRegs := 32 (only parsing).
-Notation RegFileSz := (Nat.log2_up NumRegs) (only parsing).
+Definition NumRegs := 32.
+
+Definition RegFileSz := Nat.log2 NumRegs.
 
 Definition NumInstrs := 8.
-Definition PgmSz := (Nat.log2_up NumInstrs).
+
+Definition PgmSz := Nat.log2 NumInstrs.
 
 Definition opArith : ConstT (Bit 2) := ( (* intwidth *) (natToWord 2 0))%kami.
 
@@ -44,7 +46,7 @@ Definition OpArithK := Bit 2.
 
 (* * interface Decoder *)
 Record Decoder := {
-    Decoder'mod: ModWf;
+    Decoder'mod: Mod;
     Decoder'isOp : string;
     Decoder'getOp : string;
     Decoder'getArithOp : string;
@@ -65,7 +67,7 @@ Hint Unfold Decoder'getAddr : ModuleDefs.
 
 (* * interface Executer *)
 Record Executer := {
-    Executer'mod: ModWf;
+    Executer'mod: Mod;
     Executer'execArith : string;
 }.
 
@@ -77,176 +79,14 @@ Definition MemRq := (STRUCT {
     "data" :: Bit DataSz;
     "isLoad" :: Bit 1}).
 
-(* * interface Memory *)
-Record Memory := {
-    Memory'mod: Mod;
-    Memory'doMem : string;
-}.
-
-Hint Unfold Memory'mod : ModuleDefs.
-Hint Unfold Memory'doMem : ModuleDefs.
-
-Module module'mkMemory.
-    Section Section'mkMemory.
-    Variable instancePrefix: string.
-        (* method bindings *)
-    Let (* action binding *) mem := mkRegFileFull (Bit AddrSz) (Bit DataSz) (instancePrefix--"mem").
-    (* instance methods *)
-    Let mem'sub : string := (RegFile'sub mem).
-    Let mem'upd : string := (RegFile'upd mem).
-    Local Open Scope kami_expr.
-
-    Definition mkMemoryModule: Mod :=
-         (BKMODULE {
-         Method (instancePrefix--"doMem") (req : MemRq) : (Bit DataSz) :=
-    (
-        If ((#req @% "isLoad") == $$ (* intwidth *) (natToWord 1 1)) then (
-        
-        LET addr : Bit AddrSz (* non-call varbinding *) <- (#req @% "addr") ;
-        BKCall ldval : Bit DataSz (* varbinding *) <-  (* translateCall *) mem'sub ((#addr) : Bit AddrSz)  ;
-                Ret #ldval
-        ) else (
-        
-        LET addr : Bit AddrSz (* non-call varbinding *) <- (#req @% "addr") ;
-                LET newval : Bit DataSz (* non-call varbinding *) <- (#req @% "data") ;
-        (* call expr ./ProcMemSpec.bsv:60 *) BKCall call0 : Void <-  (* translateCall *) mem'upd ((#addr) : Bit AddrSz) ((#newval) : Bit DataSz)  ;
-        BKCall placeholder : Bit DataSz (* varbinding *) <-  (* translateCall *) mem'sub ((#addr) : Bit AddrSz)  ;
-                Ret #placeholder) as retval
- ;
-        Ret #retval    )
-
-    }). (* mkMemory *)
-
-    Hint Unfold mkMemoryModule : ModuleDefs.
-(* Module mkMemory type Module#(Memory) return type Memory *)
-    Definition mkMemory := Build_Memory mkMemoryModule (instancePrefix--"doMem").
-    Hint Unfold mkMemory : ModuleDefs.
-    Hint Unfold mkMemoryModule : ModuleDefs.
-
-    End Section'mkMemory.
-End module'mkMemory.
-
-Definition mkMemory := module'mkMemory.mkMemory.
-Hint Unfold mkMemory : ModuleDefs.
-Hint Unfold module'mkMemory.mkMemory : ModuleDefs.
-Hint Unfold module'mkMemory.mkMemoryModule : ModuleDefs.
 
 (* * interface ToHost *)
 Record ToHost := {
-    ToHost'mod: ModWf;
+    ToHost'mod: Mod;
     ToHost'toHost : string;
 }.
 
 Hint Unfold ToHost'mod : ModuleDefs.
 Hint Unfold ToHost'toHost : ModuleDefs.
 
-Module module'procSpec.
-    Section Section'procSpec.
-    Variable instancePrefix: string.
-    Variable pgm: RegFile.
-    Variable dec: Decoder.
-    Variable exec: Executer.
-    Variable tohost: ToHost.
-        (* method bindings *)
-    Let pc : string := instancePrefix--"pc".
-    Let (* action binding *) rf := mkRegFileFull (Bit RegFileSz) (Bit DataSz) (instancePrefix--"rf").
-    Let (* action binding *) mem := mkMemory (instancePrefix--"mem").
-    (* instance methods *)
-    Let dec'getAddr : string := (Decoder'getAddr dec).
-    Let dec'getDst : string := (Decoder'getDst dec).
-    Let dec'getOp : string := (Decoder'getOp dec).
-    Let dec'getSrc1 : string := (Decoder'getSrc1 dec).
-    Let dec'getSrc2 : string := (Decoder'getSrc2 dec).
-    Let dec'isOp : string := (Decoder'isOp dec).
-    Let exec'execArith : string := (Executer'execArith exec).
-    Let mem'doMem : string := (Memory'doMem mem).
-    Let pgm'sub : string := (RegFile'sub pgm).
-    Let rf'sub : string := (RegFile'sub rf).
-    Let rf'upd : string := (RegFile'upd rf).
-    Let tohost'toHost : string := (ToHost'toHost tohost).
-    Local Open Scope kami_expr.
-
-    Definition procSpecModule: Mod :=
-         (BKMODULE {
-        Register pc : Bit PgmSz <-  (* intwidth *) (natToWord PgmSz 0)
-    with Rule instancePrefix--"doArith" :=
-    (
-        Read pc_v : Bit PgmSz <- pc ;
-       BKCall inst : Bit InstrSz (* varbinding *) <-  (* translateCall *) pgm'sub ((#pc_v) : Bit PgmSz)  ;
-       (* call expr ./ProcMemSpec.bsv:82 *) BKCall call2 : Bit InstrSz <-  (* translateCall *) pgm'sub ((#pc_v) : Bit PgmSz)  ;
-       (* call expr ./ProcMemSpec.bsv:82 *) BKCall call1 : Bool <-  (* translateCall *) dec'isOp ((#call2) : Bit InstrSz) (($$ (* isConstT *)opArith) : OpK)  ;
-
-        Assert(#call1) ;
-       BKCall inst : Bit InstrSz (* varbinding *) <-  (* translateCall *) pgm'sub ((#pc_v) : Bit PgmSz)  ;
-       BKCall op : OpK (* varbinding *) <-  (* translateCall *) dec'getOp ((#inst) : Bit InstrSz)  ;
-       BKCall src1 : Bit RegFileSz (* varbinding *) <-  (* translateCall *) dec'getSrc1 ((#inst) : Bit InstrSz)  ;
-       BKCall src2 : Bit RegFileSz (* varbinding *) <-  (* translateCall *) dec'getSrc2 ((#inst) : Bit InstrSz)  ;
-       BKCall dst : Bit RegFileSz (* varbinding *) <-  (* translateCall *) dec'getDst ((#inst) : Bit InstrSz)  ;
-       BKCall val1 : Bit DataSz (* varbinding *) <-  (* translateCall *) rf'sub ((#src1) : Bit RegFileSz)  ;
-       BKCall val2 : Bit DataSz (* varbinding *) <-  (* translateCall *) rf'sub ((#src2) : Bit RegFileSz)  ;
-       BKCall dval : Bit DataSz (* varbinding *) <-  (* translateCall *) exec'execArith ((#op) : OpArithK) ((#val1) : Bit DataSz) ((#val2) : Bit DataSz)  ;
-       (* call expr ./ProcMemSpec.bsv:91 *) BKCall call3 : Void <-  (* translateCall *) rf'upd ((#dst) : Bit RegFileSz) ((#dval) : Bit DataSz)  ;
-               Write pc : Bit PgmSz <- (#pc_v + $$ (* intwidth *) (natToWord PgmSz 1))  ;
-        Retv ) (* rule doArith *)
-    with Rule instancePrefix--"doLoad" :=
-    (
-        Read pc_v : Bit PgmSz <- pc ;
-       BKCall inst : Bit InstrSz (* varbinding *) <-  (* translateCall *) pgm'sub ((#pc_v) : Bit PgmSz)  ;
-       (* call expr ./ProcMemSpec.bsv:95 *) BKCall call5 : Bit InstrSz <-  (* translateCall *) pgm'sub ((#pc_v) : Bit PgmSz)  ;
-       (* call expr ./ProcMemSpec.bsv:95 *) BKCall call4 : Bool <-  (* translateCall *) dec'isOp ((#call5) : Bit InstrSz) (($$ (* isConstT *)opLd) : OpK)  ;
-
-        Assert(#call4) ;
-       BKCall inst : Bit InstrSz (* varbinding *) <-  (* translateCall *) pgm'sub ((#pc_v) : Bit PgmSz)  ;
-       BKCall addr : Bit AddrSz (* varbinding *) <-  (* translateCall *) dec'getAddr ((#inst) : Bit InstrSz)  ;
-       BKCall dst : Bit RegFileSz (* varbinding *) <-  (* translateCall *) dec'getDst ((#inst) : Bit InstrSz)  ;
-               BKCall val : Bit DataSz (* actionBinding *) <- mem'doMem ((STRUCT { "addr" ::= (#addr) ; "data" ::= ($$ (* intwidth *) (natToWord 32 0)) ; "isLoad" ::= ($$ (* intwidth *) (natToWord 1 1))  }%kami_expr) : MemRq)  ;
-       (* call expr ./ProcMemSpec.bsv:100 *) BKCall call6 : Void <-  (* translateCall *) rf'upd ((#dst) : Bit RegFileSz) ((#val) : Bit DataSz)  ;
-               Write pc : Bit PgmSz <- (#pc_v + $$ (* intwidth *) (natToWord PgmSz 1))  ;
-        Retv ) (* rule doLoad *)
-    with Rule instancePrefix--"doStore" :=
-    (
-        Read pc_v : Bit PgmSz <- pc ;
-       BKCall inst : Bit InstrSz (* varbinding *) <-  (* translateCall *) pgm'sub ((#pc_v) : Bit PgmSz)  ;
-       (* call expr ./ProcMemSpec.bsv:104 *) BKCall call8 : Bit InstrSz <-  (* translateCall *) pgm'sub ((#pc_v) : Bit PgmSz)  ;
-       (* call expr ./ProcMemSpec.bsv:104 *) BKCall call7 : Bool <-  (* translateCall *) dec'isOp ((#call8) : Bit InstrSz) (($$ (* isConstT *)opSt) : OpK)  ;
-
-        Assert(#call7) ;
-       BKCall inst : Bit InstrSz (* varbinding *) <-  (* translateCall *) pgm'sub ((#pc_v) : Bit PgmSz)  ;
-       BKCall addr : Bit AddrSz (* varbinding *) <-  (* translateCall *) dec'getAddr ((#inst) : Bit InstrSz)  ;
-       BKCall src : Bit RegFileSz (* varbinding *) <-  (* translateCall *) dec'getSrc1 ((#inst) : Bit InstrSz)  ;
-       BKCall val : Bit DataSz (* varbinding *) <-  (* translateCall *) rf'sub ((#src) : Bit RegFileSz)  ;
-               BKCall unused : Bit DataSz (* actionBinding *) <- mem'doMem ((STRUCT { "addr" ::= (#addr) ; "data" ::= (#val) ; "isLoad" ::= ($$ (* intwidth *) (natToWord 1 0))  }%kami_expr) : MemRq)  ;
-               Write pc : Bit PgmSz <- (#pc_v + $$ (* intwidth *) (natToWord PgmSz 1))  ;
-        Retv ) (* rule doStore *)
-    with Rule instancePrefix--"doHost" :=
-    (
-        Read pc_v : Bit PgmSz <- pc ;
-       BKCall inst : Bit InstrSz (* varbinding *) <-  (* translateCall *) pgm'sub ((#pc_v) : Bit PgmSz)  ;
-       (* call expr ./ProcMemSpec.bsv:113 *) BKCall call10 : Bit InstrSz <-  (* translateCall *) pgm'sub ((#pc_v) : Bit PgmSz)  ;
-       (* call expr ./ProcMemSpec.bsv:113 *) BKCall call9 : Bool <-  (* translateCall *) dec'isOp ((#call10) : Bit InstrSz) (($$ (* isConstT *)opTh) : OpK)  ;
-
-        Assert(#call9) ;
-       BKCall inst : Bit InstrSz (* varbinding *) <-  (* translateCall *) pgm'sub ((#pc_v) : Bit PgmSz)  ;
-       BKCall src1 : Bit RegFileSz (* varbinding *) <-  (* translateCall *) dec'getSrc1 ((#inst) : Bit InstrSz)  ;
-       BKCall val1 : Bit DataSz (* varbinding *) <-  (* translateCall *) rf'sub ((#src1) : Bit RegFileSz)  ;
-       (* call expr ./ProcMemSpec.bsv:118 *) BKCall call11 : Void <-  (* translateCall *) tohost'toHost ((#val1) : Bit DataSz)  ;
-               Write pc : Bit PgmSz <- (#pc_v + $$ (* intwidth *) (natToWord PgmSz 1))  ;
-        Retv ) (* rule doHost *)
-    }). (* procSpec *)
-
-    Hint Unfold procSpecModule : ModuleDefs.
-(* Module procSpec type RegFile#(Bit#(PgmSz), Bit#(InstrSz)) -> Decoder -> Executer -> ToHost -> Module#(Empty) return type Decoder *)
-(*    Definition procSpec := Build_Empty procSpecModule.
-    Hint Unfold procSpec : ModuleDefs. *)
-    Hint Unfold procSpecModule : ModuleDefs.
-
-    End Section'procSpec.
-End module'procSpec.
-
-(*
-Definition procSpec := module'procSpec.procSpec.
-Hint Unfold procSpec : ModuleDefs.
-Hint Unfold module'procSpec.procSpec : ModuleDefs.
-Hint Unfold module'procSpec.procSpecModule : ModuleDefs.
-*)
 
