example/out/ImplOk.v
@@ -1,0 +1,490 @@
+Require Import Kami.All.
+Require Import Kami.Tactics.
+Require Import Bsvtokami.
+Require Import FIFO.
+Require Import ProcMemSpec MultiCycleProc ProcDecExec.
+Require Import FinNotations.
+Require Import BKTactics.
+Require Import Decoder.
+
+Set Implicit Arguments.
+
+(*! Specifying, implementing, and verifying a very simple processor !*)
+
+(** You may want to take a look at the code in the following order:
+ * - ProcMemSpec.v: the spec of processors and memory systems
+ * - PipelinedProc.v: a 3-stage pipelined processor implementation
+ * - DecExec.v: a pipeline stage that merges the first two stages,
+ *   [decoder] and [executer].
+ * - DecExecOk.v (you are here!): correctness of [decexec] in DecExec.v
+ * - ProcMemInterm.v: an intermediate 2-stage pipelined processor 
+ * - ProcMemOk.v: a complete refinement proof
+ *)
+
+Hint Unfold Empty'mod : ModuleDefs.
+Hint Unfold NoMethods'mod : ModuleDefs.
+
+(* Here we prove that merging the first two stages ([decoder] and [executer])
+ * is correct by providing a refinement from [impl] to [spec]. *)
+Section DecExec.
+
+  Local Definition dataK := Bit ProcMemSpec.DataSz.
+  Local Definition instK := Bit ProcMemSpec.InstrSz.
+
+  Variables (kamidec: Decoder.Decoder)
+            (kamiexec: Decoder.Executer)
+            (pcInit : ConstT (Bit ProcMemSpec.PgmSz)).
+
+  Local Definition dec: ProcMemSpec.Decoder := mkDecoder kamidec "dec".
+  (* Local Definition exec: ProcMemSpec.Executer := mkExecuter kamiexec "exec". *)
+
+  Local Definition pgm := mkRegFileFull1 NumInstrs (Bit InstrSz) "pgm".
+
+  Local Definition e2wfifo := mkFIFO (Bit DataSz) "e2wfifo".
+
+  Fixpoint hideMethods m meths :=
+    match meths with
+    | meth :: meths' => hideMethods (HideMeth m meth) meths'
+    | nil => m
+    end.
+
+  Local Definition spec : Mod := 
+              hideMethods (ConcatMod
+  	                           (ConcatMod
+                                    (Empty'mod (MultiCycleProc.mkMultiCycleProc "spec" "pgm" "dec" kamiexec))
+				     (RegFile'mod pgm))
+				     (ProcMemSpec.Decoder'mod dec))
+             ("pgm-sub" :: "dec-getOp" :: "dec-getArithOp" :: "dec-getSrc1" :: "dec-getSrc2" :: "dec-getDst" :: "dec-getAddr" :: nil).
+
+
+  Local Definition impl : Mod := 
+             hideMethods (ConcatMod
+  	                           (ConcatMod
+  	                           (ConcatMod
+                                    (NoMethods'mod (ProcDecExec.mkDecExecSep "impl" "pgm" "dec" kamiexec "e2wfifo"))
+				     (RegFile'mod pgm))
+				    (ProcMemSpec.Decoder'mod dec))
+                                    (FIFO'mod e2wfifo))
+             ("e2wfifo-first" :: "e2wfifo-deq" :: "e2wfifo-clear" :: "e2wfifo-enq"
+             :: "pgm-sub" :: "dec-getOp" :: "dec-getArithOp" :: "dec-getSrc1" :: "dec-getSrc2" :: "dec-getDst" :: "dec-getAddr" :: nil).
+
+  (* What would be good invariants to prove the correctness of stage merging?
+   * For two given stages, we usually need to provide relations among states in
+   * the two stages and elements in the fifo between them.
+   *
+   * Here we describe two invariants: the first one [decexec_pc_inv] states a
+   * relation between the [pc] value and the fifo element, and the second one
+   * [decexec_d2e_inv] states that the fifo element is valid with respect to the
+   * current instruction. *)
+  Definition decexec_pc_inv
+             (impl_pcv: fullType type (SyntaxKind (Bit PgmSz)))
+             (d2efullv: fullType type (SyntaxKind Bool))
+             (d2e_pcv:      word PgmSz) :=
+             (d2efullv = true ) -> (impl_pcv = d2e_pcv ^+ $1 ).
+  
+  Definition decexec_d2e_inv
+             (pgmv: fullType type (SyntaxKind (Array NumInstrs (Bit InstrSz))))
+             (impl_pcv:         word PgmSz)
+             (d2e_pcv:      word PgmSz)
+             (d2efullv: fullType type (SyntaxKind Bool))
+             (d2e_addrv:    word AddrSz)
+             (d2e_arithopv: fullType type (SyntaxKind OpArithK))
+             (d2e_opv:      fullType type (SyntaxKind OpK))
+             (d2e_pcv:      word PgmSz)
+             (d2e_dstv:     word RegFileSz)
+             (d2e_src1v:    word RegFileSz)
+             (d2e_src2v:    word RegFileSz) :=
+    (d2efullv = true) -> (
+    let inst := evalExpr (ReadArray (Var type (SyntaxKind _) pgmv) (Var type (SyntaxKind (Bit PgmSz)) d2e_pcv )) in
+    d2e_opv = evalExpr (getOp kamidec _ inst) /\
+    d2e_arithopv = evalExpr (getArithOp kamidec _ inst) /\
+    d2e_src1v = evalExpr (getSrc1 kamidec _ inst) /\
+    d2e_src2v = evalExpr (getSrc2 kamidec _ inst) /\
+    d2e_dstv = evalExpr (getDst kamidec _ inst) /\
+    d2e_addrv = evalExpr (getAddr kamidec _ inst) /\
+    impl_pcv = (wzero PgmSz ^+ d2e_pcv ^+ $1)
+    ).
+
+
+  (* Make sure to register all invariant-related definitions in the [InvDefs]
+   * hint database, in order for Kami invariant-solving tactics to unfold them
+   * automatically. *)
+  Hint Unfold decexec_pc_inv decexec_d2e_inv: InvDefs.
+
+End DecExec.
+
+Hint Unfold dec : ModuleDefs.
+Hint Unfold pgm : ModuleDefs.
+Hint Unfold e2wfifo: ModuleDefs.
+Hint Unfold spec: ModuleDefs.
+Hint Unfold impl: ModuleDefs.
+
+Local Ltac constructor_simpl :=
+  econstructor; eauto; simpl; unfold not; intros.
+
+Local Ltac bk_discharge_wf :=
+  repeat match goal with
+         | |- @WfMod _ => constructor_simpl
+         | |- @WfConcat _ _ => constructor_simpl
+         | |- _ /\ _ => constructor_simpl
+         | |- @WfConcatActionT _ _ _ => constructor_simpl
+         | |- @WfBaseModule _ => idtac "WBM"; constructor_simpl
+         | |- @WfActionT _ _ (convertLetExprSyntax_ActionT ?e) => apply WfLetExprSyntax
+         | |- @WfActionT _ _ _ => constructor_simpl
+         | |- NoDup _ => constructor_simpl
+         | H: _ \/ _ |- _ => destruct H; subst; simpl
+         (* | |- DisjKey _ _ => discharge_DisjKey *)
+         end;
+  discharge_DisjKey.
+
+Section ImplOk.
+  Variable decoder: Decoder.Decoder.
+  Variable executer: Decoder.Executer.
+  Check dec.
+  Theorem dec_wf:
+    WfMod (ProcMemSpec.Decoder'mod (dec decoder)).
+  Proof.
+    repeat autounfold with ModuleDefs.
+    bk_discharge_wf.
+  Qed.
+
+  Theorem pgm_wf:
+    WfMod (RegFile'mod pgm).
+  Proof.
+    repeat autounfold with ModuleDefs.
+    bk_discharge_wf.
+  Qed.
+  Theorem e2wfifo_wf:
+    WfMod (FIFO'mod e2wfifo).
+  Proof.
+    repeat autounfold with ModuleDefs.
+    bk_discharge_wf.
+  Qed.
+  Theorem spec_wfmod:
+     WfMod (spec decoder executer).
+  Proof.
+    repeat autounfold with ModuleDefs.
+    discharge_wf.
+  Qed.
+
+
+  Definition specMod := (spec decoder executer).
+  Hint Unfold specMod : ModuleDefs.
+  Definition implMod := (impl decoder executer).
+  Hint Unfold implMod : ModuleDefs.
+
+  Definition specInl := flatten_inline_remove specMod.
+  Definition implInl := flatten_inline_remove implMod.
+
+  Hint Unfold specInl : ModuleDefs.
+  Hint Unfold implInl : ModuleDefs.
+
+
+Local Ltac repeat_autounfold_moduledefs := 
+  repeat autounfold with ModuleDefs ;
+  idtac "unfolded moduledefs".
+
+Ltac unfold_flatten_inline_remove :=
+  unfold hideMethods ; unfold flatten_inline_remove ;
+  unfold inlineAll_All_mod ; simpl ;
+  unfold getAllRegisters ; simpl ;
+  unfold inlineAll_All ; simpl ;
+  unfold inlineAll_Meths ; simpl ;
+  idtac "unfolding inlineSingle_Meths_pos" ;
+  try (unfold inlineSingle_Meths_pos at 11 ; simpl) ;
+  try (unfold inlineSingle_Meths_pos at 10 ; simpl) ;
+  try (unfold inlineSingle_Meths_pos at 9 ; simpl) ;
+  try (unfold inlineSingle_Meths_pos at 8 ; simpl) ;
+  try (unfold inlineSingle_Meths_pos at 7 ; simpl) ;
+  try (unfold inlineSingle_Meths_pos at 6 ; simpl) ;
+  try (unfold inlineSingle_Meths_pos at 5 ; simpl) ;
+  try (unfold inlineSingle_Meths_pos at 4 ; simpl) ;
+  try (unfold inlineSingle_Meths_pos at 3 ; simpl) ;
+  try (unfold inlineSingle_Meths_pos at 2 ; simpl) ;
+  try (unfold inlineSingle_Meths_pos at 1 ; simpl) ;
+  idtac "unfolding inlineSingle_Meths_pos" ;
+  try (unfold inlineSingle_Meths_pos at 11 ; simpl) ;
+  try (unfold inlineSingle_Meths_pos at 10 ; simpl) ;
+  try (unfold inlineSingle_Meths_pos at 9 ; simpl) ;
+  try (unfold inlineSingle_Meths_pos at 8 ; simpl) ;
+  try (unfold inlineSingle_Meths_pos at 7 ; simpl) ;
+  try (unfold inlineSingle_Meths_pos at 6 ; simpl) ;
+  try (unfold inlineSingle_Meths_pos at 5 ; simpl) ;
+  try (unfold inlineSingle_Meths_pos at 4 ; simpl) ;
+  try (unfold inlineSingle_Meths_pos at 3 ; simpl) ;
+  try (unfold inlineSingle_Meths_pos at 2 ; simpl) ;
+  try (unfold inlineSingle_Meths_pos at 1 ; simpl) ;
+  idtac "unfolding inlineSingle_Meths_pos" ;
+  try (unfold inlineSingle_Meths_pos at 11 ; simpl) ;
+  try (unfold inlineSingle_Meths_pos at 10 ; simpl) ;
+  try (unfold inlineSingle_Meths_pos at 9 ; simpl) ;
+  try (unfold inlineSingle_Meths_pos at 8 ; simpl) ;
+  try (unfold inlineSingle_Meths_pos at 7 ; simpl) ;
+  try (unfold inlineSingle_Meths_pos at 6 ; simpl) ;
+  try (unfold inlineSingle_Meths_pos at 5 ; simpl) ;
+  try (unfold inlineSingle_Meths_pos at 4 ; simpl) ;
+  try (unfold inlineSingle_Meths_pos at 3 ; simpl) ;
+  try (unfold inlineSingle_Meths_pos at 2 ; simpl) ;
+  try (unfold inlineSingle_Meths_pos at 1 ; simpl) ;
+  idtac "unfolding inlineSingle_Meths_pos" ;
+  try (unfold inlineSingle_Meths_pos at 11 ; simpl) ;
+  try (unfold inlineSingle_Meths_pos at 10 ; simpl) ;
+  try (unfold inlineSingle_Meths_pos at 9 ; simpl) ;
+  try (unfold inlineSingle_Meths_pos at 8 ; simpl) ;
+  try (unfold inlineSingle_Meths_pos at 7 ; simpl) ;
+  try (unfold inlineSingle_Meths_pos at 6 ; simpl) ;
+  try (unfold inlineSingle_Meths_pos at 5 ; simpl) ;
+  try (unfold inlineSingle_Meths_pos at 4 ; simpl) ;
+  try (unfold inlineSingle_Meths_pos at 3 ; simpl) ;
+  try (unfold inlineSingle_Meths_pos at 2 ; simpl) ;
+  try (unfold inlineSingle_Meths_pos at 1 ; simpl) ;
+  idtac "unfolding inlineAll_Rules" ;
+  unfold inlineAll_Rules ; unfold Datatypes.length ; unfold range ; simpl ;
+  unfold inlineSingle_Rules_pos ; simpl ;
+  unfold removeHides ;
+  unfold getRegisters ; unfold getRules ; unfold getMethods ;
+  unfold in_dec ; unfold getBool ; unfold negb ; unfold filter ; simpl ;
+  idtac "flatten_inline_remove".
+
+Ltac discharge_flatten_inline_remove :=
+  time repeat_autounfold_moduledefs ;
+  time unfold_flatten_inline_remove.  
+
+(*
+Theorem implInlWf:
+  WfBaseModule implInl.
+Proof.
+  idtac "implInlWf".
+  discharge_flatten_inline_remove.
+  idtac "discharging wf"
+  time discharge_wf.
+Qed.
+ 
+Theorem specInlWf:
+  WfBaseModule specInl.
+Proof.
+  idtac "specInlWf".
+  discharge_flatten_inline_remove.
+  idtac "discharging wf"
+  time discharge_wf.
+Qed.
+
+*)
+
+Record mySimRel (dec : Decoder) (iregs sregs: RegsT): Prop :=
+ {
+   pgmv: (Fin.t NumInstrs -> word DataSz) ;
+
+   impl_d2e_validv: bool ;
+   impl_pcv: word PgmSz ;
+   impl_e2w_validv: fullType type (SyntaxKind (Bit 1)) ;
+   impl_e2w_valv: fullType type (SyntaxKind (Bit DataSz)) ;
+   impl_rf_v: fullType type (SyntaxKind (Array NumRegs (Bit DataSz))) ;
+
+   spec_pcv: word PgmSz ;
+   spec_rf_v: (Fin.t NumRegs -> word DataSz) ;
+   spec_stagev: word 2 ;
+   spec_d2e_opv: fullType type (SyntaxKind OpK) ;
+   spec_d2e_arithopv: fullType type (SyntaxKind OpArithK) ;
+   spec_d2e_src1v: word RegFileSz ;
+   spec_d2e_src2v: word RegFileSz ;
+   spec_d2e_dstv: word RegFileSz ;
+   spec_d2e_addrv: word AddrSz ;
+   spec_d2e_valv: word DataSz ;
+   spec_d2e_pgmv: (Fin.t NumInstrs -> word InstrSz) ;
+   spec_e2w_dstv: word RegFileSz ;
+   spec_e2w_valv: word DataSz ;
+
+   impl_d2e_addrv    : word AddrSz ;
+   impl_d2e_arithopv : fullType type (SyntaxKind OpArithK) ;
+   impl_d2e_opv      : fullType type (SyntaxKind OpK) ;
+   impl_d2e_pcv      : word PgmSz ;
+   impl_d2e_dstv     : word RegFileSz ;
+   impl_d2e_src1v    : word RegFileSz ;
+   impl_d2e_src2v    : word RegFileSz ;
+
+   Hiregs: iregs =
+   ("impl-pc", existT _ (SyntaxKind (Bit PgmSz)) impl_pcv)
+   :: ("impl-d2e_valid", existT _ (SyntaxKind Bool) impl_d2e_validv)
+   :: ("impl-d2e_pc", existT _ (SyntaxKind (Bit PgmSz)) impl_d2e_pcv)
+   :: ("impl-d2e_op", existT _ (SyntaxKind OpK) impl_d2e_opv)
+   :: ("impl-d2e_arithOp", existT _ (SyntaxKind OpArithK) impl_d2e_arithopv)
+   :: ("impl-d2e_src1", existT _ (SyntaxKind (Bit RegFileSz)) impl_d2e_src1v)
+   :: ("impl-d2e_src2", existT _ (SyntaxKind (Bit RegFileSz)) impl_d2e_src2v)
+   :: ("impl-d2e_dst", existT _ (SyntaxKind (Bit RegFileSz)) impl_d2e_dstv)
+   :: ("impl-rf", existT _ (SyntaxKind (Array NumRegs (Bit DataSz))) impl_rf_v)
+   :: ("pgm-rfreg", existT _ (SyntaxKind (Array NumInstrs (Bit InstrSz))) pgmv)
+   :: ("e2wfifo-valid", existT (fullType type) (SyntaxKind (Bit 1)) impl_e2w_validv)
+   :: ("e2wfifo-v", existT (fullType type) (SyntaxKind (Bit DataSz)) impl_e2w_valv)
+   :: nil ;
+
+   Hsregs: sregs =
+   ("spec-pc", existT _ (SyntaxKind (Bit PgmSz)) spec_pcv)
+  :: ("spec-rf", existT _ (SyntaxKind (Array NumRegs (Bit DataSz))) spec_rf_v)
+     :: ("spec-stage", existT _ (SyntaxKind (Bit 2)) spec_stagev)
+        :: ("spec-d2e_op", existT _ (SyntaxKind OpK) spec_d2e_opv)
+           :: ("spec-d2e_arithOp", existT _ (SyntaxKind OpArithK) spec_d2e_arithopv)
+              :: ("spec-d2e_src1", existT _ (SyntaxKind (Bit RegFileSz)) spec_d2e_src1v)
+                 :: ("spec-d2e_src2", existT _ (SyntaxKind (Bit RegFileSz)) spec_d2e_src2v)
+                    :: ("spec-d2e_dst", existT _ (SyntaxKind (Bit RegFileSz)) spec_d2e_dstv)
+                       :: ("spec-d2e_addr", existT _ (SyntaxKind (Bit AddrSz)) spec_d2e_addrv)
+                          :: ("spec-e2w_dst", existT _ (SyntaxKind (Bit RegFileSz)) spec_e2w_dstv)
+                             :: ("spec-e2w_val", existT _ (SyntaxKind (Bit DataSz)) spec_e2w_valv)
+                                :: ("pgm-rfreg", existT _ (SyntaxKind (Array NumInstrs (Bit InstrSz))) spec_d2e_pgmv)
+				   :: nil ;
+
+   Hpcinv: (impl_d2e_validv = true ) -> (impl_pcv = impl_d2e_pcv ^+ $1 /\ spec_pcv = impl_d2e_pcv) ;
+   Hpcinv_decode: (impl_d2e_validv = false ) -> (impl_pcv = spec_pcv) ;
+   Hdeinv: decexec_d2e_inv dec pgmv impl_pcv
+               impl_d2e_pcv
+               impl_d2e_validv
+               impl_d2e_addrv
+               impl_d2e_arithopv
+               impl_d2e_opv
+               impl_d2e_pcv
+               impl_d2e_dstv 
+               impl_d2e_src1v
+               impl_d2e_src2v ;
+
+   Hstageinv: (impl_d2e_validv = false ) -> spec_stagev = wzero 2 ;
+   Hstageinv_exec: (impl_d2e_validv = true /\ impl_e2w_validv = (natToWord 1 0) ) -> spec_stagev = (natToWord 2 1) ;
+   Hstageinv_wv: (impl_e2w_validv = (natToWord 1 1) ) -> spec_stagev = (natToWord 2 2) ;
+   He2w_val:   impl_e2w_validv = (natToWord 1 1) ->  impl_e2w_valv = spec_e2w_valv ;
+
+ }.
+
+
+Ltac andb_true_intro_split := apply andb_true_intro; split.
+
+Lemma findStr A B (dec: forall a1 a2, {a1 = a2} + {a1 <> a2}):
+  forall (ls: list (A * B)),
+  forall x, In x ls <->
+            In x (filter (fun t => getBool (dec (fst x) (fst t))) ls).
+Proof.
+  induction ls; simpl; split; auto; intros.
+  - destruct H; [subst|]; auto.
+    + destruct (dec (fst x) (fst x)) ; simpl in *; tauto.
+    + apply IHls in H.
+      destruct (dec (fst x) (fst a)) ; simpl in *; auto.
+  - destruct (dec (fst x) (fst a)) ; simpl in *.
+    + destruct H; auto.
+      apply IHls in H; auto.
+    + eapply IHls in H; eauto.
+Qed.
+
+Ltac foo :=
+    subst;
+    repeat
+      (match goal with
+       | H:DisjKey _ _
+         |- _ =>
+         apply DisjKeyWeak_same in H;
+           [ unfold DisjKeyWeak in H; simpl in H | apply string_dec ]
+       | H: In ?x ?ls |- _ =>
+         apply (findStr string_dec) in H; simpl in H; destruct H; [|exfalso; auto]
+       | H:False |- _ => exfalso; apply H
+       | H:(?A, ?B) = (?P, ?Q)
+         |- _ =>
+         let H1 := fresh in
+         let H2 := fresh in
+         pose proof (f_equal fst H) as H1; pose proof (f_equal snd H) as H2; simpl in H1, H2;
+           clear H
+       | H:?A = ?A |- _ => clear H
+       | H:(?a ++ ?b)%string = (?a ++ ?c)%string |- _ => rewrite append_remove_prefix in H; subst
+       | H:(?a ++ ?b)%string = (?c ++ ?b)%string |- _ => rewrite append_remove_suffix in H; subst
+       | H:existT ?a ?b ?c1 = existT ?a ?b ?c2
+         |- _ => apply Eqdep.EqdepTheory.inj_pair2 in H
+       | H:?A = ?B |- _ => discriminate
+       | H: ?x && ?y = true |- _ => rewrite andb_true_iff in H
+       | H: negb ?x = true |- _ => apply negb_true_iff in H
+       | H: negb ?x = false |- _ => apply negb_false_iff in H
+       | H: ?x /\ ?y |- _ => destruct H
+       | H:SemAction _ (convertLetExprSyntax_ActionT ?e) _ _ _ _
+         |- _ => apply convertLetExprSyntax_ActionT_full in H; dest
+       | |- _ -> _ => intro
+       | |- ?a = ?a => reflexivity
+       end; subst).
+
+Ltac discharge_whatever :=
+  repeat (match goal with
+          | H: _ |- Forall2 ?p ?l1 ?l2 => apply Forall2_cons; simpl
+          | H: _ |- Forall2 ?p nil nil => apply Forall2_nil
+          | H: _ |- ?a /\ ?b => split
+          | H: _ |- _ :: _ = _ :: _ => repeat f_equal
+          | H: _ |- ?a = ?a => reflexivity
+          | H: _ |- exists _, _ => exists eq_refl
+          end).
+
+Theorem impl_ok:
+    TraceInclusion implInl specInl 
+(*
+                   (getModWf {| baseModule := implInl ; wfBaseModule := ltac:(apply implInlWf) |})
+                   (getModWf {| baseModule := specInl ; wfBaseModule := ltac:(apply specInlWf) |})
+*).
+  Proof.
+  idtac "impl_ok".
+  discharge_flatten_inline_remove.
+  idtac "apply simulationGeneral".
+  time discharge_simulation (mySimRel decoder).
+  + reflexivity.
+  + reflexivity.
+  + foo.
+  + foo.
+
+  + (* decode rule *)
+    right. exists "spec-doDecode". eexists. split.
+    * left. trivial.
+    * (* reads spec *) eexists. (* updates spec *) eexists. split.
+     ** discharge_SemAction.
+     apply negb_true_iff in H1. simpl.
+     rewrite H1 in Hstageinv.
+     specialize (Hstageinv eq_refl). rewrite Hstageinv.
+     simpl. reflexivity.
+     ** simpl.
+     evar (impl_d2e_validv0 : bool).
+     evar (impl_pcv0 : word PgmSz).
+     econstructor 1 with (impl_d2e_validv := impl_d2e_validv0)
+                         (pgmv := x6) (impl_pcv := impl_pcv0) (spec_pcv := spec_pcv).
+     *** trivial.
+     *** repeat (f_equal).
+        instantiate (impl_d2e_validv0 := true).
+
+        instantiate (impl_pcv0 := wzero PgmSz ^+ x1 ^+ $1).
+        unfold impl_pcv0. reflexivity. 
+        unfold impl_d2e_validv0. reflexivity.
+     *** repeat f_equal.
+     *** unfold impl_d2e_validv0. intro. unfold impl_pcv0. rewrite wzero_wplus.
+        split. reflexivity.
+        apply negb_true_iff in H1. rewrite H1 in Hpcinv_decode. specialize (Hpcinv_decode eq_refl).
+        rewrite Hpcinv_decode. reflexivity.
+     *** foo.
+     *** unfold decexec_d2e_inv. unfold impl_d2e_validv0. foo. simpl. repeat split.
+     *** unfold impl_d2e_validv0. intro. inv H.
+     *** trivial.
+     *** Compute implInl. intro. Search (_ -> False). apply except. inv H. inv H0. admit.
+     *** intro. Search (False -> _). apply except. inv H. inv H0. admit.
+
+  + (* arith rule *)
+    right. exists "spec-doExec". eexists. split.
+  * right. left. trivial.
+    * (* reads spec *) eexists. (* updates spec *) eexists. split.
+     **  discharge_SemAction.
+        foo. specialize (Hpcinv eq_refl). destruct Hpcinv.
+        (* specialize (Hstageinv_exec eq_refl). *)
+        admit.
+     ** simpl.
+evar (impl_d2e_validv0 : bool).
+econstructor 1 with (impl_d2e_validv := impl_d2e_validv0).
+     *** trivial.
+     *** repeat f_equal. unfold impl_d2e_validv0. trivial.
+     *** repeat f_equal.
+     *** unfold impl_d2e_validv0. foo.
+         specialize (Hpcinv eq_refl). apply Hpcinv.
+     *** foo.
+     *** unfold decexec_d2e_inv. unfold decexec_d2e_inv in Hdeinv. foo. specialize (Hdeinv eq_refl).
+         foo. repeat split.
+     *** foo.
+     *** trivial.
+     *** intro. simpl.  
+Qed.
+End ImplOk.
