example/out/MultiCycleProc.v
@@ -1,0 +1,108 @@
+Require Import Bool String List Arith.
+Require Import Omega.
+Require Import Kami.All.
+Require Import Bsvtokami.
+Require Import Decoder.
+Require Import ProcMemSpec.
+
+Module module'mkMultiCycleProc.
+    Section Section'mkMultiCycleProc.
+    Variable instancePrefix: string.
+    Variable pgm: string.
+    Variable dec: string.
+    Variable exec: Decoder.Executer.
+        (* method bindings *)
+    Let pc : string := instancePrefix--"pc".
+    Let stage : string := instancePrefix--"stage".
+    Let d2e_op : string := instancePrefix--"d2e_op".
+    Let d2e_arithOp : string := instancePrefix--"d2e_arithOp".
+    Let d2e_src1 : string := instancePrefix--"d2e_src1".
+    Let d2e_src2 : string := instancePrefix--"d2e_src2".
+    Let d2e_dst : string := instancePrefix--"d2e_dst".
+    Let d2e_addr : string := instancePrefix--"d2e_addr".
+    Let e2w_val : string := instancePrefix--"e2w_val".
+    (* instance methods *)
+    Let dec'getDst : string := (dec--"getDst").
+    Let dec'getOp : string := (dec--"getOp").
+    Let dec'getSrc1 : string := (dec--"getSrc1").
+    Let dec'getSrc2 : string := (dec--"getSrc2").
+    Let pgm'sub : string := (pgm--"sub").
+    Local Open Scope kami_expr.
+
+    Definition mkMultiCycleProcModule: ModWf :=
+         (MOD_WF {
+        Register (instancePrefix--"pc") : Bit PgmSz <- Default
+    with Register (instancePrefix--"rf") : Array NumRegs (Bit DataSz) <- Default
+    with Register (instancePrefix--"stage") : Bit 2 <- Default
+    with Register (instancePrefix--"d2e_op") : OpK <- Default
+    with Register (instancePrefix--"d2e_arithOp") : OpArithK <- Default
+    with Register (instancePrefix--"d2e_src1") : Bit RegFileSz <- Default
+    with Register (instancePrefix--"d2e_src2") : Bit RegFileSz <- Default
+    with Register (instancePrefix--"d2e_dst") : Bit RegFileSz <- Default
+    with Register (instancePrefix--"d2e_addr") : Bit AddrSz <- Default
+    with Register (instancePrefix--"e2w_dst") : Bit RegFileSz <- Default
+    with Register (instancePrefix--"e2w_val") : Bit DataSz <- Default
+    with Rule instancePrefix--"doDecode" :=
+    (
+        Read pc_v : Bit PgmSz <- pc ;
+        Read stage_v : Bit 2 <- stage ;
+
+        Assert((#stage_v == $$ (* intwidth *) (natToWord 2 0))) ;
+       Call inst : Bit InstrSz (* varbinding *) <-  (* translateCall *) pgm'sub ((#pc_v) : Bit PgmSz)  ;
+       (* call expr ./ProcMemSpec.bsv:95 *) Call call1 : OpK <-  (* translateCall *) dec'getOp ((#inst) : Bit InstrSz)  ;
+               Write d2e_op : OpK <- #call1  ;
+       (* call expr ./ProcMemSpec.bsv:96 *) Call call2 : Bit RegFileSz <-  (* translateCall *) dec'getSrc1 ((#inst) : Bit InstrSz)  ;
+               Write d2e_src1 <- #call2  ;
+       (* call expr ./ProcMemSpec.bsv:97 *) Call call3 : Bit RegFileSz <-  (* translateCall *) dec'getSrc2 ((#inst) : Bit InstrSz)  ;
+               Write d2e_src2 : Bit RegFileSz <- #call3  ;
+       (* call expr ./ProcMemSpec.bsv:98 *) Call call4 : Bit RegFileSz <-  (* translateCall *) dec'getDst ((#inst) : Bit InstrSz)  ;
+               Write d2e_dst : Bit RegFileSz <- #call4  ;
+               Write stage : Bit 2 <- $$ (* intwidth *) (natToWord 2 1)  ;
+        Retv ) (* rule doDecode *)
+
+    with Rule instancePrefix--"doExec" :=
+    (
+        Read d2e_dst_v : Bit RegFileSz <- d2e_dst ;
+        Read d2e_op_v : OpK <- d2e_op ;
+        Read d2e_src1_v : Bit RegFileSz <- d2e_src1 ;
+        Read d2e_src2_v : Bit RegFileSz <- d2e_src2 ;
+        Read stage_v : Bit 2 <- stage ;
+
+        Assert((#stage_v == $$ (* intwidth *) (natToWord 2 1))) ;
+       Read rf_v : Array NumRegs (Bit DataSz) <- (instancePrefix--"rf") ;
+       LET val1 : Bit DataSz (* varbinding *) <-  #rf_v @[#d2e_src1_v]  ;
+       LET val2 : Bit DataSz (* varbinding *) <-  #rf_v @[#d2e_src2_v]  ;
+       LET dval : Bit DataSz (* varbinding *) <-  (execArith exec _ d2e_op_v val1 val2)  ;
+               Write instancePrefix--"e2w_dst" : Bit RegFileSz <- #d2e_dst_v  ;
+               Write instancePrefix--"e2w_val" : Bit DataSz <- #dval  ;
+               Write stage : Bit 2 <- $$ (* intwidth *) (natToWord 2 2)  ;
+        Retv ) (* rule doExec *)
+    with Rule instancePrefix--"doWriteBack" :=
+    (
+        Read e2w_dst_v : Bit RegFileSz <- instancePrefix--"e2w_dst" ;
+        Read e2w_val_v : Bit DataSz <- instancePrefix--"e2w_val" ;
+        Read pc_v : Bit PgmSz <- pc ;
+        Read stage_v : Bit 2 <- stage ;
+
+        Assert((#stage_v == $$ (* intwidth *) (natToWord 2 2))) ;
+        Read rf_v : Array NumRegs (Bit DataSz) <- (instancePrefix--"rf") ;
+	LET rf_v : Array NumRegs (Bit DataSz) <- #rf_v @[#e2w_dst_v <- #e2w_val_v ]  ;
+        Write (instancePrefix--"rf") : Array NumRegs (Bit DataSz) <-  #rf_v ;
+        Write pc : Bit PgmSz <- (#pc_v + $$ (* intwidth *) (natToWord PgmSz 1))  ;
+        Write stage : Bit 2 <- $$ (* intwidth *) (natToWord 2 0)  ;
+        Retv ) (* rule doWriteBack *)
+    }). (* mkMultiCycleProc *)
+
+    Hint Unfold mkMultiCycleProcModule : ModuleDefs.
+
+    Definition mkMultiCycleProc := Build_Empty mkMultiCycleProcModule.
+    Hint Unfold mkMultiCycleProc : ModuleDefs.
+    Hint Unfold mkMultiCycleProcModule : ModuleDefs.
+
+    End Section'mkMultiCycleProc.
+End module'mkMultiCycleProc.
+
+Definition mkMultiCycleProc := module'mkMultiCycleProc.mkMultiCycleProc.
+Hint Unfold mkMultiCycleProc : ModuleDefs.
+Hint Unfold module'mkMultiCycleProc.mkMultiCycleProc : ModuleDefs.
+Hint Unfold module'mkMultiCycleProc.mkMultiCycleProcModule : ModuleDefs.
